A12Kernel.lean
@@ -101,6 +101,7 @@ import A12Kernel.Elaboration.StringComputation
 import A12Kernel.Elaboration.StringComputationTable
 import A12Kernel.Elaboration.StringComputationRun
 import A12Kernel.Elaboration.StringComputationRunRelation
+import A12Kernel.Elaboration.StringComputationRunResult
 import A12Kernel.Elaboration.EnumerationComputation
 import A12Kernel.Elaboration.EnumerationFirstFilledComputation
 import A12Kernel.Elaboration.NumericValidation
